Parser improvements, but this approach is wrong

parser/Parser.fst
@@ -1,7 +1,8 @@
 module Parser
 
 (*
-A very simple parser combinator library.
+A parser combinator library with very simple implementations,
+but complex types. :(
 
 Parsers are functions that take a string and return a parse_result which
 contains either a user-specified value and the remaining portion of the string,
@@ -20,7 +21,7 @@ type parse_result 'a =
 
 // The type of a parser 
 type parser 'a = (x:string) -> Tot (r:(parse_result 'a){ParseError? r ||
-  is_substring (Success?.rest r) x})
+  is_suffix (Success?.rest r) x})
 
 // Transform the result of a single parser
 let parse_apply #a #b (f:a->b) (x:(parser a)) : (parser b) =
@@ -38,7 +39,7 @@ let parse_seq #a #b (x:(parser a)) (y:(parser b)) : Tot (parser (a*b)) =
     match (y rest) with
       | ParseError e2 a2 -> ParseError e2 a2
       | Success t2 r2 -> 
-        ( substring_transitivity r2 rest input;
+        ( suffix_transitivity r2 rest input;
           Success (t1, t2) r2 )
 
 //  <,> to create pairs
@@ -53,7 +54,7 @@ let parse_list #a (x:(parser (list a))) (y:(parser (list a))) : Tot (parser (lis
   | Success t1 rest -> match (y rest) with
       | ParseError e2 a2 -> ParseError e2 a2 
       | Success t2 r2 -> 
-        (substring_transitivity r2 rest input;
+        (suffix_transitivity r2 rest input;
          Success (FStar.List.Tot.append t1 t2) r2)
 
 // TODO: how to combine this with the above?
@@ -65,11 +66,11 @@ let parse_nonempty_list #a (x:(parser (z:(list a){Cons? z}))) (y:(parser (list a
   | Success t1 rest -> match (y rest) with
       | ParseError e2 a2 -> ParseError e2 a2 
       | Success t2 r2 -> 
-        (substring_transitivity r2 rest input;
+        (suffix_transitivity r2 rest input;
          Success (FStar.List.Tot.append t1 t2) r2)
  
-// <::> to create lists
-let op_Less_Colon_Colon_Greater (#a:Type) (x:parser (list a)) (y:parser (list a)) =
+// <@> to create lists
+let op_Less_At_Greater (#a:Type) (x:parser (list a)) (y:parser (list a)) =
   parse_list #a x y
 
 // Explicitly combine the parse results from two types into a third
@@ -80,7 +81,7 @@ let parse_comb #a #b #c (x:(parser a)) (f: a -> b -> Tot c) (y:(parser b)) : Tot
   | Success t1 rest -> match (y rest) with
       | ParseError e2 a2 -> ParseError e2 a2
       | Success t2 r2 -> 
-        (substring_transitivity r2 rest input;
+        (suffix_transitivity r2 rest input;
         Success (f t1 t2) r2)
 
 // Don't think we can create a ternary operator, but somebody could define their own
@@ -109,9 +110,21 @@ let parse_either #a (x:(parser a)) (y:(parser a)) : Tot (parser a) =
      | Success t2 r2 -> Success t2 r2 
      | ParseError e2 a2 -> or_of_reasons e1 e2 input
 
+let parse_either_relax #a (#pa:(a -> Type)) (#pb:(a -> Type)) 
+   (x:(parser (z:a{pa z}))) 
+   (y:(parser (z:a{pb z}))) : Tot (parser (z:a{pa z \/ pb z})) =
+  fun (input:string) -> 
+  match (x input) with
+  | Success t1 rest -> Success t1 rest
+  | ParseError e1 a1 -> match (y input) with
+     | Success t2 r2 -> Success t2 r2 
+     | ParseError e2 a2 -> or_of_reasons e1 e2 input
+
 // <|> to create alternatives
-let op_Less_Bar_Greater (#a:Type) (x:(parser a)) (y:(parser a)) =
-  parse_either x y
+let op_Less_Bar_Greater #a (#pa:(a -> Type)) (#pb:(a -> Type)) 
+   (x:(parser (z:a{pa z}))) 
+   (y:(parser (z:a{pb z}))) = 
+  parse_either_relax x y
 
 type left_right 'a 'b =
  | Left : left:'a -> left_right 'a 'b
@@ -132,19 +145,20 @@ let parse_lr #a #b (x:(parser a)) (y:(parser b)) : Tot (parser (left_right a b))
 // (Previous approach: define proper and improper parsers, but then we'd have to have
 // make multiple version of the above combinators, probably?)
 let rec parse_star_aux #a (input:string) (x:parser a) (prev_a:list a) 
-: Tot ((list a)*(remaining:string{is_substring remaining input})) 
+: Tot ((list a)*(remaining:string{is_suffix remaining input})) 
   (decreases (strlen input)) =
   match (x input) with
   | ParseError _ at -> 
-     substring_is_reflexive input;
+     suffix_is_reflexive input;
      ((List.Tot.rev prev_a),input)
   | Success v rest -> 
      if rest = input then ((List.Tot.rev prev_a),input)
-       else ( substring_is_shorter rest input;
+       else ( suffix_is_shorter rest input;
+              suffix_is_substring rest input;
               proper_substring rest input;
               let next_match = parse_star_aux rest x (v :: prev_a) in
-                ( substring_transitivity (snd next_match) rest input;
-                  assert( is_substring (snd next_match) input );
+                ( suffix_transitivity (snd next_match) rest input;
+                  assert( is_suffix (snd next_match) input );
                   // OK, this is dumb, F* knows about (snd next_match) but it
                   // can't apply that to intrinsic type of the pair without
                   // me spelling it out for it.
@@ -162,6 +176,22 @@ let listify #a (x:a) : y:(list a){Cons? y} = [x]
 let parse_plus #a (x:(parser a)) : Tot (parser (z:(list a){Cons? z})) =
   parse_nonempty_list (parse_apply listify x) (parse_star x)
 
+// Parse one or one of the given parser, returned as an option
+let parse_option #a (x:(parser a)) : Tot (parser (option a)) =
+  fun (input:string) ->
+  match (x input) with
+  | Success v rest -> Success (Some v) rest
+  | ParseError _ _ -> 
+    suffix_is_reflexive input;
+    Success None input
+
+// Rename the failure condition on parsing
+let parse_rename #a (e:string) (x:(parser a)) : Tot (parser a) =
+  fun (input:string) ->
+  match (x input) with
+  | Success v rest -> Success v rest
+  | ParseError _ at -> ParseError e at
+  
 (*
   Parsers for basic types
 *)
@@ -173,24 +203,84 @@ let literal (a:string) : Tot (parser (m:string{m=a})) =
      ParseError (sprintf "literal '%s'" a) input
   else let m = sub input 0 (strlen a) in
      if m = a then
-        Success m (sub input (strlen a) ((strlen input) - (strlen a)))
+        Success m (suffix input (strlen a))
      else
         ParseError (sprintf "literal '%s'" a) input
 
 // Return a specific value when the string is matched
-let literal_of #b (a:string) (v:b) (input:string) : Tot (parse_result (m:b{m==v})) =
+let literal_of #b (a:string) (v:b) : Tot (parser (m:b{m==v})) =
+  fun (input:string) ->
   match literal a input with
   | ParseError expected at -> ParseError expected at
   | Success _ rest -> Success v rest
 
-type digit_string = (x:string{x = "0" || x = "1" || x = "2" || x = "3" || x = "4" || x = "5" || x = "6" || x = "7" || x = "8" || x = "9"})
+// Return the value inside of the given brackets
+let brackets #a (lbracket:string) (x:parser a) (rbracket:string) : Tot (parser a) =
+  parse_comb 
+    (literal lbracket)
+    (fun t1 t2 -> t2 )
+    (parse_comb
+      x
+      (fun t2 t3 -> t2 )
+      (literal rbracket))
 
+type digit_string = (x:string{x = "0" \/ x = "1" \/ x = "2" \/ x = "3" \/ x = "4" \/ x = "5" \/ x = "6" \/ x = "7" \/ x = "8" \/ x = "9"})
+
+// This definition fails if one of the possibilities is missing!
+// ... or out of order.
 let digit : (parser digit_string) =
-    literal "0" <|> literal "1" <|> literal "2" <|> literal "3"
-  
+    parse_rename "digit" (literal "0" <|> literal "1" <|> literal "2" <|> literal "3" <|> literal "4" <|> literal "5" <|> literal "6" <|> literal "7" <|> literal "8" <|> literal "9")
 
-let integer (input:string) : Tot (parse_result int) = 
-  
+let digit_string_to_int (d:digit_string) : int = 
+  match d with
+  | "0" -> 0
+  | "1" -> 1
+  | "2" -> 2
+  | "3" -> 3
+  | "4" -> 4
+  | "5" -> 5
+  | "6" -> 6
+  | "7" -> 7
+  | "8" -> 8
+  | "9" -> 9
+
+let rec dl_to_int_aux (remaining_digits : list digit_string) (prev:int) : int =
+  match remaining_digits with
+  | [] -> prev
+  | hd :: tl -> dl_to_int_aux tl ((op_Multiply 10 prev) + (digit_string_to_int hd))
+     
+let dl_to_int (d : list digit_string{Cons?d}) : int =
+  dl_to_int_aux d 0
+
+// TODO: prove that dl_to_int is the inverse of printing an unsigned integer
+
+// Parse an unsigned decimal 
+let unsigned_integer : parser int = 
+    parse_rename "unsigned integer" 
+      (parse_apply dl_to_int (parse_plus digit))
+
+// Parse a signed decimal (only - is recognized, not +)
+let signed_integer : parser int = 
+    parse_rename "integer"
+      (parse_comb 
+        (parse_option (literal "-"))
+        (fun o i -> match o with
+         | Some _ -> op_Multiply (-1) i
+         | None -> i)
+        unsigned_integer)
+        
+// Consume any space and go on to the next parser
+// TODO: work on any whitespace characters
+let space #a (x:parser a) : parser a =
+    parse_comb
+      (parse_star (literal " "))
+      (fun ws result -> result)
+      x
+
+
+
+
+
 
 
   
