parser/StringLemmas.fsti
@@ -2,11 +2,29 @@ module StringLemmas
 
 open FStar.String
 
-val is_prefix (a:string) (b:string) : bool
-val is_suffix (a:string) (b:string) : bool
-val is_substring (a:string) (b:string) : prop
+// These predicates are defined in the interface
+// so that when we take a prefix or suffix it is recognizable as uch.
 
-let suffix (b:string) (n:nat{n <= strlen b}) : (x:string{n = strlen x}) =
+let is_prefix (a:string) (b:string) : bool = 
+  if strlen a > strlen b then false else
+  (sub b 0 (strlen a)) = a
+
+let is_suffix (a:string) (b:string) : bool = 
+  if strlen a > strlen b then false else
+  (sub b (strlen b - strlen a) (strlen a)) = a
+
+let is_substring (a:string) (b:string) : prop = 
+  exists (i:nat) (n:nat). i + n <= strlen b /\ (sub b i n) == a 
+
+val prefix_is_substring (a:string) (b:string) :
+  Lemma (requires (is_prefix a b))
+        (ensures (is_substring a b))
+
+val suffix_is_substring (a:string) (b:string) :
+  Lemma (requires (is_suffix a b))
+        (ensures (is_substring a b))
+
+let suffix (b:string) (n:nat{n <= strlen b}) : (x:string{strlen x = n /\ is_suffix x b}) =
   (sub b (strlen b - n) n)
 
 // If two strings have zero length, they are equal.
@@ -17,20 +35,39 @@ val all_strings_of_length_zero_are_equal (s:string{strlen s=0}) (t:string{strlen
 val substring_of_length_is_equal (s:string) 
  : Lemma (ensures (sub s 0 (strlen s)) = s )
 
-// All strings are prefixes of themeselves
+// Reflexive properties
 val prefix_is_reflexive (s:string)
+ : Lemma (ensures is_prefix s s)
+
+val suffix_is_reflexive (s:string)
+ : Lemma (ensures is_suffix s s)
+
+val substring_is_reflexive (s:string)
  : Lemma (ensures is_substring s s)
 
 // The substring relationship imposes an order on string length
+val prefix_is_shorter (a:string) (b:string) 
+ : Lemma (requires (is_prefix a b))
+         (ensures (strlen a) <= (strlen b) )
+
+val suffix_is_shorter (a:string) (b:string) 
+ : Lemma (requires (is_suffix a b))
+         (ensures (strlen a) <= (strlen b) )
+
 val substring_is_shorter (a:string) (b:string) 
  : Lemma (requires (is_substring a b))
          (ensures (strlen a) <= (strlen b) )
 
-// Prefix of prefix 
+// The relation between substrings and nested substrings,
+// and special cases for prefixes and suffixes
+val substring_of_substring_is_substring (s:string) 
+   (p1:nat) (n1:nat{p1+n1 <= strlen s}) 
+   (p2:nat) (n2:nat{p2+n2 <= n1})
+ : Lemma (ensures (sub s (p1+p2) n2) == (sub (sub s p1 n1) p2 n2))
+
 val prefix_of_prefix_is_prefix (s:string) (x:nat{strlen s >= x}) (y:nat{y <= x})
  : Lemma (ensures (sub s 0 y) == (sub (sub s 0 x) 0 y))
  
-// Suffix of suffix
 val suffix_of_suffix_is_suffix (s:string) (x:nat{strlen s >= x}) (y:nat{y <= x})
  : Lemma (ensures (suffix s y) == (suffix (suffix s x) y))
 
